Oops, this was not actually merged in Iris.
Revert "Bump Iris (persistent mapsto)."

This reverts commit 7e770adaa0d0755ea9e8d38fb1b43a7faae6e6f6.

theories/examples/stack/refinement.v
@@ -8,10 +8,24 @@ Definition stackN := nroot.@"stack".
 Section proof.
   Context `{relocG Σ}.
 
+  (** The "partial pointsto" proposition is duplicable *)
+  Local Instance istk_fromand (istk : loc) (w : val) :
+    FromSep (∃ q, istk ↦{q} w) (∃ q, istk ↦{q} w) (∃ q, istk ↦{q} w).
+  Proof.
+    rewrite /FromSep. iIntros "[$ _]".
+  Qed.
+  Local Instance istk_intoand (istk : loc) (w : val) :
+    IntoSep (∃ q, istk ↦{q} w) (∃ q, istk ↦{q} w) (∃ q, istk ↦{q} w).
+  Proof.
+    rewrite /IntoSep /=. iDestruct 1 as (q) "[H1 H2]".
+    iSplitL "H1"; eauto with iFrame.
+  Qed.
+
   Fixpoint stack_contents (v1 : loc) (ls : list val) :=
     match ls with
-    | [] => v1 ↦□ NONEV
-    | h::tl => ∃ (z1 : loc), v1 ↦□ SOMEV (h, #z1) ∗ stack_contents z1 tl
+    | [] => ∃ q, v1 ↦{q} NONEV
+    | h::tl => ∃ (z1 : loc) q, v1 ↦{q} SOMEV (h, #z1) ∗
+                 stack_contents z1 tl
     end%I.
 
   Definition stack_link (A : lrel Σ) (v1 : loc) (v2 : val) :=
@@ -19,32 +33,45 @@ Section proof.
         stack_contents v1 ls1 ∗ is_stack v2 ls2 ∗
         [∗ list] v1;v2 ∈ ls1;ls2, A v1 v2)%I.
 
-  Global Instance stack_contents_persistent v1 ls :
-    Persistent (stack_contents v1 ls).
-  Proof. revert v1. induction ls; apply _. Qed.
+  (** Actually, the whole `stack_contents` predicate is duplicable *)
+  Local Instance stack_contents_intoand (istk : loc) (ls : list val) :
+    IntoSep (stack_contents istk ls) (stack_contents istk ls) (stack_contents istk ls).
+  Proof.
+    rewrite /IntoSep /=.
+    revert istk. induction ls as [|h ls]; intros istk; simpl.
+    - apply istk_intoand.
+    - iDestruct 1 as (z1 q) "[Histk Hc]".
+      rewrite IHls. iDestruct "Hc" as "[Hc1 Hc2]". iDestruct "Histk" as "[Histk1 Histk2]".
+      iSplitL "Hc1 Histk1"; iExists _, (q/2)%Qp; by iFrame.
+  Qed.
 
   Lemma stack_contents_agree istk ls ls' :
     stack_contents istk ls -∗ stack_contents istk ls' -∗ ⌜ls = ls'⌝.
   Proof.
     revert istk ls'. induction ls as [|h ls]; intros istk ls'; simpl.
-    - iIntros "#Histk".
+    - iDestruct 1 as (q) "Histk".
       destruct ls' as [|h' ls']; first by eauto.
-      simpl. iDestruct 1 as (z) "[Histk' _]".
-      iDestruct (mapsto_agree with "Histk' Histk") as %Hfoo.
+      simpl. iDestruct 1 as (z q') "[Histk' _]".
+      iDestruct (gen_heap.mapsto_agree with "Histk' Histk") as %Hfoo.
       exfalso. naive_solver.
-    - iDestruct 1 as (z) "[Histk Hls]".
+    - iDestruct 1 as (z q) "[Histk Hls]".
       destruct ls' as [|h' ls']; simpl.
-      + iIntros "Histk'".
-        iDestruct (mapsto_agree with "Histk' Histk") as %Hfoo.
+      + iDestruct 1 as (q') "Histk'".
+        iDestruct (gen_heap.mapsto_agree with "Histk' Histk") as %Hfoo.
         exfalso. naive_solver.
-      + iDestruct 1 as (z') "[Histk' Hls']".
-        iDestruct (mapsto_agree with "Histk' Histk") as %Hfoo; simplify_eq/=.
+      + iDestruct 1 as (z' q') "[Histk' Hls']".
+        iDestruct (gen_heap.mapsto_agree with "Histk' Histk") as %Hfoo. simplify_eq/=.
         iDestruct (IHls with "Hls Hls'") as %Hbar. simplify_eq/=.
         eauto.
   Qed.
 
   Definition sinv (A : lrel Σ) stk stk' : iProp Σ :=
     (∃ (istk : loc), stk  ↦ #istk ∗ stack_link A istk stk')%I.
+
+  Ltac close_sinv Hcl asn :=
+    iMod (Hcl with asn) as "_";
+    [iNext; rewrite /sinv; iExists _;
+         (by iFrame || iFrame; iExists _,_; by eauto with iFrame) |]; try iModIntro.
 
   Lemma FG_CG_push_refinement N st st' (A : lrel Σ) (v v' : val) :
     N ## relocN →
@@ -61,8 +88,7 @@ Section proof.
     iInv N as (isk) "(>Hstk & Hlnk)" "Hclose".
     iExists _. iFrame.
     iModIntro. iNext. iIntros "Hstk".
-    iMod ("Hclose" with "[Hlnk Hstk]") as "_".
-    { iExists _. by iFrame. }
+    close_sinv "Hclose" "[Hlnk Hstk]".
     rel_pures_l.
     rel_alloc_l nstk as "Hnstk".
     rel_cmpxchg_l_atomic.
@@ -71,19 +97,17 @@ Section proof.
     iModIntro. iSplit.
     - (* CmpXchg fails *)
       iIntros (?); iNext; iIntros "Hstk".
-      iMod ("Hclose" with "[Hlnk Hstk]") as "_".
-      { iExists _. iFrame. }
+      close_sinv "Hclose" "[Hlnk Hstk]".
       rel_pures_l. rel_rec_l. by iApply "IH".
     - (* CmpXchg succeeds *)
       iIntros (?). simplify_eq/=. iNext. iIntros "Hstk".
-      iMod (mapsto_persist with "Hnstk") as "Hnstk".
       rewrite /stack_link. iDestruct "Hlnk" as (ls1 ls2) "(Hls1 & Hls2 & #HA)".
       rel_apply_r (refines_CG_push_r with "Hls2").
       iIntros "Hls2".
       iMod ("Hclose" with "[-]").
       { iNext. rewrite {2}/sinv. iExists _. iFrame.
         iExists (v::ls1),_. simpl. iFrame "Hls2 Hvv HA".
-        iExists _. iFrame. }
+        iExists _,_. iFrame. }
       rel_pures_l. rel_values.
   Qed.
 
@@ -101,40 +125,38 @@ Section proof.
     iExists _. iFrame "Hstk".
     iModIntro. iNext. iIntros "Hstk /=".
     rel_pures_l. rel_rec_l.
-    iDestruct "Hlnk" as (ls1 ls2) "(#Hls1 & Hls2 & #HA)".
-    destruct ls1 as [|h1 ls1]; iSimpl in "Hls1".
+    iDestruct "Hlnk" as (ls1 ls2) "(Hls1 & Hls2 & #HA)".
+    iDestruct "Hls1" as "[Histk1 Histk2]".
+    destruct ls1 as [|h1 ls1]; iSimpl in "Histk1".
     - iDestruct (big_sepL2_length with "HA") as %Hfoo.
       assert (ls2 = []) as -> by (apply length_zero_iff_nil; done). clear Hfoo.
       rel_apply_r (refines_CG_pop_fail_r with "Hls2").
-      iIntros "Hls2". simpl in *.
-      iMod ("Hclose" with "[Hstk Hls2]") as "_".
-      { iExists _. iFrame. iExists [], []. iFrame; auto. }
-      rel_load_l.
+      iIntros "Hls2".
+      close_sinv "Hclose" "[Histk2 Hstk Hls2]".
+      iDestruct "Histk1" as (q) "Histk'". rel_load_l.
       rel_pures_l. rel_values.
       iModIntro. iExists _,_. eauto.
-    - iDestruct "Hls1" as (z1) "[Hls1 Hrest]".
-      iMod ("Hclose" with "[Hstk Hls2]") as "_".
-      { iExists _. iFrame. iExists (h1 :: ls1), _. simpl. auto. }
+    - iDestruct "Histk1" as (z1 q) "[Histk1 Hrest]".
+      close_sinv "Hclose" "[Histk2 Hstk Hls2]".
       rel_load_l. rel_pures_l.
       rel_cmpxchg_l_atomic.
       iInv N as (istk') "(>Hstk & Hlnk)" "Hclose".
       iModIntro. iExists _. iFrame "Hstk". iSplit.
       + iIntros (?). iNext. iIntros "Hstk".
-        iMod ("Hclose" with "[Hstk Hlnk]") as "_".
-        { iExists _. iFrame. }
+        close_sinv "Hclose" "[Hstk Hlnk]".
         rel_pures_l. iApply "IH".
       + iIntros (?). simplify_eq/=. iNext.
         iIntros "Hstk". rel_pures_l.
         iDestruct "Hlnk" as (ls1' ls2') "(Hc2 & Hst & #HA')".
-        iAssert (stack_contents istk (h1::ls1)) with "[Hls1]" as "{Hls1} Hls1".
-        { simpl. iExists _. auto. }
-        iDestruct (stack_contents_agree with "Hls1 Hc2") as %<-.
+        iDestruct "Hrest" as "[Hrest Hz1]".
+        iAssert (stack_contents istk (h1::ls1)) with "[Histk1 Hrest]" as "Histk1".
+        { simpl. iExists _,_. by iFrame. }
+        iDestruct (stack_contents_agree with "Histk1 Hc2") as %<-.
         iClear "HA".
         rewrite big_sepL2_cons_inv_l. iDestruct "HA'" as (h2 l2' ->) "[Hh HA]".
         rel_apply_r (refines_CG_pop_suc_r with "Hst").
         iIntros "Hst".
-        iMod ("Hclose" with "[-]") as "_".
-        { iExists _. iFrame. iExists _, _; auto. }
+        close_sinv "Hclose" "[-]".
         rel_values. iModIntro. iExists _,_; eauto.
   Qed.
 
@@ -157,7 +179,6 @@ Section proof.
       rel_alloc_r st' as "Hst'". rel_pures_r.
       rel_apply_r refines_newlock_r. iIntros (l) "Hl". rel_pures_r.
       rel_values.
-      iMod (mapsto_persist with "Hisk") as "#Hisk".
       iMod (inv_alloc (stackN.@(st,(#st', l)%V)) _ (sinv A st (#st', l)%V) with "[-]")
         as "#Hinv".
       { iNext. iExists _. iFrame. iExists [],[]. simpl.
